Dinic/Compute_Blocking_Residual.thy
@@ -1,0 +1,151 @@
+theory Compute_Blocking_Residual
+  imports DFS_Collect_Backtrack_Example Compute_Blocking_Simple "HOL-Library.Product_Lexorder"
+begin
+
+global_interpretation blocking_simple: blocking_simple where insert = vset_insert and
+ sel = sel and  vset_empty = vset_empty and  diff = vset_diff and
+ lookup = lookup and empty = map_empty and delete=delete and isin = isin and t_set=t_set
+and update=update and adjmap_inv = adj_inv and vset_delete= vset_delete
+and vset_inv = vset_inv and union=vset_union and inter=vset_inter 
+and flow_lookup = lookup
+and flow_empty = Leaf
+and flow_update=update
+and flow_delete=delete
+and flow_invar=adj_inv
+and G = G and
+t = t and
+s = s and
+find_path = find_path and
+u = u
+for G s t find_path u
+defines blocking_simple_loop=blocking_simple.compute_blocking_loop_impl
+and     blocking_simple_initial=blocking_simple.initial_state
+and add_flow_simple=blocking_simple.add_flow
+and delete_edge=blocking_simple.delete_edge
+  by(auto intro!: blocking_simple.intro
+           simp add: dfs.Graph.Pair_Graph_Specs_axioms  dfs.set_ops.Set2_axioms
+                      M.Map_axioms[simplified RBT_Set.empty_def adj_inv_def[symmetric]])
+
+definition "find_path F s t = 
+   (if neighbourhood F s = vset_empty then None
+    else let final_state = dfs_del_dead_impl F t ( dfs_backtrack_initial_state s)
+         in  (case return final_state of NotReachable \<Rightarrow> None |
+                                         Reachable    \<Rightarrow> 
+              Some (rev (stack final_state), backtrack final_state)))"
+
+value "find_path G 0 10"
+value "find_path G 0 6"
+
+value "blocking_simple_initial G"
+value "find_path G 0 10"
+value "blocking_simple_loop 0 10 find_path (\<lambda> e. 4) (blocking_simple_initial G)"
+value "inorder (flow (blocking_simple_loop 0 10 find_path (\<lambda> e. 4) (blocking_simple_initial G)))"
+
+hide_const G edges
+
+lemma find_path_correct:
+assumes "dfs.Graph.graph_inv F" "dfs.Graph.finite_graph F" "dfs.Graph.finite_vsets F" "s \<noteq> t"
+shows "\<exists>p. vwalk_bet (dfs.Graph.digraph_abs F) s p t \<Longrightarrow>
+       \<exists>p del. vwalk_bet (dfs.Graph.digraph_abs F) s p t \<and> find_path F s t = Some (p, del)"
+       (is "?asm1 \<Longrightarrow> ?thesis1")
+      "find_path F s t = Some (p, dlt) \<Longrightarrow>
+       acyc (dfs.Graph.digraph_abs F) \<Longrightarrow>
+       vwalk_bet (dfs.Graph.digraph_abs F) s p t \<and>
+       distinct p \<and>
+       (\<forall>e\<in>set dlt. \<nexists>p. e \<in> set (edges_of_vwalk p) \<and> vwalk_bet (dfs.Graph.digraph_abs F) s p t)"
+       (is "?asm2 \<Longrightarrow> ?asm3 \<Longrightarrow> ?thesis2")
+proof(all \<open>cases "neighbourhood F s = vset_empty"\<close>)
+ show  "?asm1 \<Longrightarrow> ?thesis1" if asy: "neighbourhood F s = vset_empty"
+   using assms(4) dfs.Graph.vset.set.set_empty vwalk_then_edge[of "dfs.Graph.digraph_abs F" s _  t] 
+   by(unfold dfs.Graph.are_connected_abs[OF assms(1), symmetric] asy) blast
+  show  "?asm2 \<Longrightarrow> ?asm3 \<Longrightarrow> ?thesis2"  if asy: "neighbourhood F s = vset_empty"
+    using asy by(simp add: find_path_def)
+  assume s_neighb_non_empty:"neighbourhood F s \<noteq> vset_empty"
+  have DFS_axioms: "DFS.DFS_axioms isin t_set adj_inv vset_empty vset_inv lookup F s"
+    using RBT_Set.empty_def Tree2.eq_set_tree_empty assms(1,2,3)  s_neighb_non_empty
+    by(auto intro:dfs.Graph.neighbourhood_absD simp add: dfs.DFS_axioms_def)
+  have dfs_thms: "DFS_thms map_empty RBT_Map.delete vset_insert isin t_set sel update adj_inv vset_empty vset_delete vset_inv
+     vset_union vset_inter vset_diff lookup F s"
+    by(auto intro!: DFS_thms.intro DFS_thms_axioms.intro simp add: dfs.DFS_axioms DFS_axioms)
+  have same_final_state: "dfs_del_dead_impl F t ( dfs_backtrack_initial_state s) =
+                         dfs.DFS_collect_backtrack F t ( dfs_backtrack_initial_state s)"
+    by(simp add: dfs_del_dead_impl_def dfs_backtrack_initial_state_def
+                 DFS_thms.DFS_collect_backtrack_impl_same_on_initial[OF dfs_thms]) 
+  have same_final_as_ordinary: "to_ordinary_DFS_state 
+                    (dfs.DFS_collect_backtrack F t ( dfs_backtrack_initial_state s)) =
+                    dfs.DFS F t ( dfs.initial_state s)"
+    using DFS_thms.same_as_old_dfs_on_initial[OF dfs_thms]
+    by(simp add: dfs_backtrack_initial_state_def)
+  note DFS_correct_1 = DFS_thms.DFS_correct_1_weak[OF dfs_thms]
+  note DFS_correct_2 = DFS_thms.DFS_correct_2[OF dfs_thms]
+  show  "?asm1 \<Longrightarrow> ?thesis1"
+  proof(goal_cases)
+    case 1
+    hence dfs_reachable:"DFS_state.return (dfs.DFS F t (dfs.initial_state s)) = Reachable"
+      using DFS_correct_1 return.exhaust by blast
+    define final_state where "final_state = dfs_del_dead_impl F t ( dfs_backtrack_initial_state s)"
+    have dfs_backtrack_reachable: "return final_state =  Reachable"
+      using  dfs_reachable same_final_as_ordinary[symmetric]  same_final_state
+      by(auto simp add: final_state_def)
+    show ?case 
+    proof(rule exI[of _ "rev (stack final_state)"], rule exI[of _ "backtrack final_state"],
+            rule conjI, goal_cases)
+      case 2
+      then show ?case
+        using s_neighb_non_empty dfs_backtrack_reachable 
+        by(auto simp add: find_path_def  final_state_def split: return.split)
+    next
+      case 1
+      then show ?case 
+        using  DFS_correct_2[OF dfs_reachable] same_final_as_ordinary[symmetric]
+        by(simp add: final_state_def  same_final_state) 
+    qed 
+  qed
+  show  "?asm2 \<Longrightarrow> ?asm3 \<Longrightarrow> ?thesis2"
+  proof(goal_cases)
+    case 1
+     define final_state where "final_state = dfs_del_dead_impl F t ( dfs_backtrack_initial_state s)"
+     have dfs_backtrack_result: "return final_state =  Reachable" "rev (stack final_state) = p" 
+                                "backtrack final_state = dlt"
+     apply(all \<open>rule case_split[of "DFS_Collect_Backtrack_Example.neighbourhood F s = vset_empty"]\<close>)
+     apply(all \<open>rule return.exhaust[of "DFS_backtrack_state.return (dfs_del_dead_impl
+                         F t (dfs_backtrack_initial_state s))"]\<close>)
+     using "1"(1) 
+     by(auto simp add: final_state_def find_path_def) 
+   have "vwalk_bet (dfs.Graph.digraph_abs F) s p t"
+     using DFS_correct_2[of t]  dfs_backtrack_result(1) dfs_backtrack_result(2)       
+     by(auto simp add: final_state_def same_final_state same_final_as_ordinary[symmetric])
+   moreover have "distinct p" 
+     using DFS_thms.invar_seen_stack_holds[OF dfs_thms 
+                                    DFS_thms.initial_state_props(6,1,3)[OF dfs_thms], of t]
+     by(simp add: dfs.invar_seen_stack_def same_final_as_ordinary[symmetric]
+                   dfs_backtrack_result(2)[symmetric] final_state_def same_final_state)
+   moreover have "e\<in>set dlt \<Longrightarrow>
+                  \<nexists>p. e \<in> set (edges_of_vwalk p) \<and> vwalk_bet (dfs.Graph.digraph_abs F) s p t" for e
+     using  same_final_state  "1"(2) DFS_thms.dfs_backtrack_final(5)[OF dfs_thms, of t]       
+     by(simp add: dfs.invar_dfs_backtrack_5_def acyc_def  dfs_backtrack_initial_state_def 
+                  final_state_def  dfs_backtrack_result(2,3)[symmetric])     
+   ultimately show ?case by auto
+ qed
+qed
+
+interpretation blocking_simple_thms: blocking_simple_thms where insert = vset_insert and
+ sel = sel and  vset_empty = vset_empty and  diff = vset_diff and
+ lookup = lookup and empty = map_empty and delete=delete and isin = isin and t_set=t_set
+and update=update and adjmap_inv = adj_inv and vset_delete= vset_delete
+and vset_inv = vset_inv and union=vset_union and inter=vset_inter 
+and flow_lookup = lookup
+and flow_empty = Leaf
+and flow_update=update
+and flow_delete=delete
+and flow_invar=adj_inv
+and G = G and
+t = t and
+s = s and
+find_path = find_path and
+u = u
+for G s t u
+  apply(auto intro!: blocking_simple_thms.intro) 
+  apply (simp add: blocking_simple.flow_map.Map_axioms blocking_simple.intro
+      dfs.Graph.Pair_Graph_Specs_axioms dfs.set_ops.Set2_axioms)
+  apply(rule blocking_simple_thms_axioms.intro)
